extraction/theories/BetaEq.v
@@ -1,0 +1,245 @@
+From ConCert.Extraction Require Import Aux.
+From ConCert.Extraction Require Import ClosedAux.
+From ConCert.Extraction Require Import ExAst.
+From ConCert.Extraction Require Import ExTyping.
+From ConCert.Extraction Require Import Optimize.
+From ConCert.Extraction Require Import WcbvEvalAux.
+From Coq Require Import Arith.
+From Coq Require Import Bool.
+From Coq Require Import Morphisms.
+From Coq Require Import String.
+From Coq Require Import List.
+From Coq Require Import Psatz.
+From Coq Require Import RelationClasses.
+From Equations Require Import Equations.
+From MetaCoq.Erasure Require Import EAstUtils.
+From MetaCoq.Erasure Require Import ECSubst.
+From MetaCoq.Erasure Require Import EInduction.
+From MetaCoq.Erasure Require Import ELiftSubst.
+From MetaCoq.Erasure Require Import EWcbvEval.
+From MetaCoq.Template Require Import utils.
+
+Import ListNotations.
+
+Import EAstUtils.
+
+Reserved Infix "β=" (at level 70, right associativity).
+
+Inductive betaeq : term -> term -> Prop :=
+| betaeq_beta na body arg : tApp (tLambda na body) arg β= body{0 := arg}
+| betaeq_evar i ts ts' :
+    betaeq_terms ts ts' ->
+    tEvar i ts β= tEvar i ts'
+| betaeq_lambda na body body' :
+    body β= body' ->
+    tLambda na body β= tLambda na body'
+| betaeq_let_in na val val' body body' :
+    val β= val' ->
+    body β= body' ->
+    tLetIn na val body β= tLetIn na val' body'
+| betaeq_app hd hd' arg arg' :
+    hd β= hd' ->
+    arg β= arg' ->
+    tApp hd arg β= tApp hd' arg'
+| betaeq_case p disc disc' brs brs' :
+    disc β= disc' ->
+    betaeq_branches brs brs' ->
+    tCase p disc brs β= tCase p disc' brs'
+| betaeq_proj p t t' :
+    t β= t' ->
+    tProj p t β= tProj p t'
+| betaeq_fix defs defs' i :
+    betaeq_defs defs defs' ->
+    tFix defs i β= tFix defs' i
+| betaeq_cofix defs defs' i :
+    betaeq_defs defs defs' ->
+    tCoFix defs i β= tCoFix defs' i
+| betaeq_refl t : t β= t
+| betaeq_sym t t' : t β= t' -> t' β= t
+| betaeq_trans a b c :
+    a β= b ->
+    b β= c ->
+    a β= c
+
+with betaeq_terms : list term -> list term -> Prop :=
+| betaeq_terms_nil : betaeq_terms [] []
+| betaeq_terms_cons t t' ts ts' :
+    t β= t' ->
+    betaeq_terms ts ts' ->
+    betaeq_terms (t :: ts) (t' :: ts')
+
+with betaeq_branches : list (nat × term) -> list (nat × term) -> Prop :=
+| betaeq_branches_nil : betaeq_branches [] []
+| betaeq_branches_cons b b' brs brs' :
+    b.1 = b'.1 ->
+    b.2 β= b'.2 ->
+    betaeq_branches brs brs' ->
+    betaeq_branches (b :: brs) (b' :: brs')
+
+with betaeq_defs : mfixpoint term -> mfixpoint term -> Prop :=
+| betaeq_defs_nil : betaeq_defs [] []
+| betaeq_defs_cons d d' defs defs' :
+    dname d = dname d' ->
+    dbody d β= dbody d' ->
+    rarg d = rarg d' ->
+    betaeq_defs defs defs' ->
+    betaeq_defs
+      (d :: defs)
+      (d' :: defs')
+
+where "t β= t'" := (betaeq t t').
+
+Derive Signature for betaeq.
+
+Hint Constructors betaeq betaeq_terms betaeq_branches betaeq_defs : beta.
+
+Lemma betaeq_terms_Forall2 ts ts' :
+  betaeq_terms ts ts' <-> Forall2 betaeq ts ts'.
+Proof. split; induction 1; eauto with beta. Qed.
+
+Lemma betaeq_branches_Forall2 brs brs' :
+  betaeq_branches brs brs' <->
+  Forall2 (fun b b' => b.1 = b'.1 /\ b.2 β= b'.2) brs brs'.
+Proof.
+  split; induction 1; eauto with beta.
+  destruct H.
+  eauto with beta.
+Qed.
+
+Lemma betaeq_defs_Forall2 defs defs' :
+  betaeq_defs defs defs' <->
+  Forall2 (fun d d' => dname d = dname d' /\
+                       dbody d β= dbody d' /\
+                       rarg d = rarg d') defs defs'.
+Proof.
+  split; induction 1; eauto with beta.
+  destruct H as (? & ? & ?); eauto with beta.
+Qed.
+
+Ltac beta_to_all :=
+  rewrite -> ?betaeq_terms_Forall2 in *;
+  rewrite -> ?betaeq_branches_Forall2 in *;
+  rewrite -> ?betaeq_defs_Forall2 in *.
+
+Ltac all_to_beta :=
+  rewrite <- ?betaeq_terms_Forall2 in *;
+  rewrite <- ?betaeq_branches_Forall2 in *;
+  rewrite <- ?betaeq_defs_Forall2 in *.
+
+Scheme betaeq_mind := Induction for betaeq Sort Prop
+  with betaeq_terms_mind := Induction for betaeq_terms Sort Prop
+  with betaeq_branches_mind := Induction for betaeq_branches Sort Prop
+  with betaeq_defs_mind := Induction for betaeq_defs Sort Prop.
+
+(*
+Definition betaeq_forall_list_ind
+           (P : term -> term -> Prop)
+           (Hbetal : forall (na : name) (body arg sub : term),
+               body{0 := arg} β= sub ->
+               P (body {0 := arg}) sub ->
+               P (tApp (tLambda na body) arg) sub)
+           (Hbetar : forall (na : name) (body arg sub : term),
+               sub β= body {0 := arg} ->
+               P sub (body {0 := arg}) ->
+               P sub (tApp (tLambda na body) arg))
+           (Hbox : P tBox tBox)
+           (Hrel : forall i : nat, P (tRel i) (tRel i))
+           (Hvar : forall id : ident, P (tVar id) (tVar id))
+           (Hevar : forall (i : nat) (ts ts' : list term),
+               Forall2 (fun t t' => t β= t' /\ P t t') ts ts' ->
+               P (tEvar i ts) (tEvar i ts'))
+           (Hlambda : forall (na : name) (body body' : term),
+               body β= body' ->
+               P body body' ->
+               P (tLambda na body) (tLambda na body'))
+           (Hletin : forall (na : name) (val val' body body' : term),
+               val β= val' ->
+               P val val' ->
+               body β= body' ->
+               P body body' ->
+               P (tLetIn na val body) (tLetIn na val' body'))
+           (Happ : forall hd hd' arg arg' : term,
+               hd β= hd' ->
+               P hd hd' ->
+               arg β= arg' ->
+               P arg arg' ->
+               P (tApp hd arg) (tApp hd' arg'))
+           (Hconst : forall kn : kername, P (tConst kn) (tConst kn))
+           (Hconstruct : forall (ind : inductive) (c : nat),
+               P (tConstruct ind c) (tConstruct ind c))
+           (Hcase : forall (p : inductive × nat) (disc disc' : term)
+                           (brs brs' : list (nat × term)),
+               disc β= disc' ->
+               P disc disc' ->
+               Forall2 (fun '(ar, t) '(ar', t') => ar = ar' /\ t β= t' /\ P t t') brs brs' ->
+               P (tCase p disc brs) (tCase p disc' brs'))
+           (Hproj : forall (p : projection) (t t' : term),
+               t β= t' ->
+               P t t' ->
+               P (tProj p t) (tProj p t'))
+           (Hfix : forall (defs defs' : list (def term)) (i : nat),
+               Forall2
+                 (fun d d' =>
+                    dname d = dname d' /\
+                    rarg d = rarg d' /\
+                    dbody d β= dbody d' /\
+                    P (dbody d) (dbody d')) defs defs' ->
+               P (tFix defs i) (tFix defs' i))
+           (Hcofix : forall (defs defs' : list (def term)) (i : nat),
+               Forall2
+                 (fun d d' =>
+                    dname d = dname d' /\
+                    rarg d = rarg d' /\
+                    dbody d β= dbody d' /\
+                    P (dbody d) (dbody d')) defs defs' ->
+               P (tCoFix defs i) (tCoFix defs' i)) :
+  forall t t', t β= t' -> P t t'.
+Proof.
+  fix ind 3.
+  intros t t' beq.
+  destruct beq;
+    try solve [match goal with [ H : _ |- _ ] =>
+                               match type of H with
+                                 forall t t', t β= t' -> _ => fail 1
+                               | _ => eapply H
+                               end end; eauto].
+  - apply Hevar.
+    clear -H ind.
+    revert ts ts' H.
+    fix f 3.
+    destruct 1; constructor; [|auto].
+    split; [assumption|].
+    apply ind; auto.
+  - apply Hcase; [assumption|apply ind; auto|].
+    clear -H ind.
+    revert brs brs' H.
+    fix f 3.
+    destruct 1; constructor; [|auto].
+    destruct b, b'.
+    split; [assumption|].
+    split; [assumption|].
+    apply ind; auto.
+  - apply Hfix.
+    clear -H ind.
+    revert defs defs' H.
+    fix f 3.
+    destruct 1; constructor; [|auto].
+    split; [assumption|].
+    split; [assumption|].
+    split; [assumption|].
+    apply ind; auto.
+  - apply Hcofix.
+    clear -H ind.
+    revert defs defs' H.
+    fix f 3.
+    destruct 1; constructor; [|auto].
+    cbn.
+    split; [assumption|].
+    split; [assumption|].
+    split; [assumption|].
+    apply ind; auto.
+Defined.
+*)
+
+Instance Equivalence_betaeq : Equivalence betaeq.
+Proof. constructor; eauto with beta. Qed.
