extraction/theories/ScbvEval.v
@@ -1,0 +1,135 @@
+From ConCert.Extraction Require Import Aux.
+From ConCert.Extraction Require Import ClosedAux.
+From ConCert.Extraction Require Import ExAst.
+From ConCert.Extraction Require Import ExTyping.
+From ConCert.Extraction Require Import Optimize.
+From ConCert.Extraction Require Import WcbvEvalAux.
+From Coq Require Import Arith.
+From Coq Require Import Bool.
+From Coq Require Import Morphisms.
+From Coq Require Import String.
+From Coq Require Import List.
+From Coq Require Import Psatz.
+From Coq Require Import RelationClasses.
+From Equations Require Import Equations.
+From MetaCoq.Erasure Require Import EAst.
+From MetaCoq.Erasure Require Import EAstUtils.
+From MetaCoq.Erasure Require Import ECSubst.
+From MetaCoq.Erasure Require Import EInduction.
+From MetaCoq.Erasure Require Import ELiftSubst.
+From MetaCoq.Erasure Require Import ETyping.
+From MetaCoq.Erasure Require Import EWcbvEval.
+From MetaCoq.Template Require Import utils.
+
+Import ListNotations.
+
+Import EAstUtils.
+
+Section seval.
+Context (Σ : global_declarations).
+Inductive eval : term -> term -> Prop :=
+(** Reductions *)
+| eval_box a t t' :
+    eval a tBox ->
+    eval t t' ->
+    eval (tApp a t) tBox
+
+(** Beta *)
+| eval_beta f na b a a' res :
+    eval f (tLambda na b) ->
+    eval a a' ->
+    eval (csubst a' 0 b) res ->
+    eval (tApp f a) res
+
+(** Let *)
+| eval_zeta na b0 b0' b1 res :
+    eval b0 b0' ->
+    eval (csubst b0' 0 b1) res ->
+    eval (tLetIn na b0 b1) res
+
+(** Case *)
+| eval_iota ind pars discr c args brs res :
+    eval discr (mkApps (tConstruct ind c) args) ->
+    eval (iota_red pars c args brs) res ->
+    eval (tCase (ind, pars) discr brs) res
+
+(** Singleton case on a proof *)
+| eval_iota_sing ind pars discr brs n f res :
+    eval discr tBox ->
+    brs = [ (n,f) ] ->
+    eval (mkApps f (repeat tBox n)) res ->
+    eval (tCase (ind, pars) discr brs) res
+
+(** Fix unfolding, with guard *)
+| eval_fix f mfix idx argsv a av narg fn res :
+    eval f (mkApps (tFix mfix idx) argsv) ->
+    eval a av ->
+    cunfold_fix mfix idx = Some (narg, fn) ->
+    #|argsv| = narg ->
+             is_constructor_app_or_box av ->
+             eval (tApp (mkApps fn argsv) av) res ->
+             eval (tApp f a) res
+
+(** Fix stuck, with guard *)
+| eval_fix_value f mfix idx argsv a av narg fn :
+    eval f (mkApps (tFix mfix idx) argsv) ->
+    eval a av ->
+    cunfold_fix mfix idx = Some (narg, fn) ->
+    (#|argsv| <> narg \/ (#|argsv| = narg /\ ~~is_constructor_app_or_box av)) ->
+    eval (tApp f a) (tApp (mkApps (tFix mfix idx) argsv) av)
+
+(** CoFix-case unfolding *)
+| red_cofix_case ip mfix idx args narg fn brs res :
+    cunfold_cofix mfix idx = Some (narg, fn) ->
+    eval (tCase ip (mkApps fn args) brs) res ->
+    eval (tCase ip (mkApps (tCoFix mfix idx) args) brs) res
+
+(** CoFix-proj unfolding *)
+| red_cofix_proj p mfix idx args narg fn res :
+    cunfold_cofix mfix idx = Some (narg, fn) ->
+    eval (tProj p (mkApps fn args)) res ->
+    eval (tProj p (mkApps (tCoFix mfix idx) args)) res
+
+(** Constant unfolding *)
+| eval_delta c decl body (isdecl : declared_constant Σ c decl) res :
+    decl.(cst_body) = Some body ->
+    eval body res ->
+    eval (tConst c) res
+
+(** Proj *)
+| eval_proj i pars arg discr args k res :
+    eval discr (mkApps (tConstruct i k) args) ->
+    eval (List.nth (pars + arg) args tDummy) res ->
+    eval (tProj (i, pars, arg) discr) res
+
+(** Proj *)
+| eval_proj_box i pars arg discr :
+    eval discr tBox ->
+    eval (tProj (i, pars, arg) discr) tBox
+
+(** Atoms (non redex-producing heads) applied to values are values *)
+| eval_app_cong f f' a a' :
+    eval f f' ->
+    ~~ (isLambda f' || isFixApp f' || isBox f') ->
+    eval a a' ->
+    eval (tApp f a) (tApp f' a')
+
+| eval_atom_rel i : eval (tRel i) (tRel i)
+| eval_atom_box : eval tBox tBox
+| eval_atom_lambda na body body' :
+    eval body body' ->
+    eval (tLambda na body) (tLambda na body')
+| eval_atom_construct ind c : eval (tConstruct ind c) (tConstruct ind c)
+| eval_atom_fix defs defs' n :
+
+    Forall2 eval (map dbody defs) (map dbody defs')
+
+(** Evars complicate reasoning due to the embedded substitution, we skip
+      them for now *)
+(* | eval_evar n l l' : *)
+(*     Forall2 eval l l' -> *)
+(*     eval (tEvar n l) (tEvar n l') *)
+
+
+(** Atoms are values (includes abstractions, cofixpoints and constructors) *)
+| eval_atom t : atom t -> eval t t.
